Add examples

Test/concurrency/10-SequenceInvariant.dfy
@@ -1,25 +1,8 @@
 // RUN: %dafny /compile:0 "%s" > "%t"
 // RUN: %diff "%s.expect" "%t"
 
-// This program shows how to model a program that concurrently increments a counter by a fixed amount.
-//
-// Rust-like source code:
-// fn incrementer(counter: Arc<AtomicIsize>, remaining: &mut isize)
-//   requires *remaining == 10
-//   ensures *remaining == 0
-// {
-//     let mut i = 0;
-//     while i < 10 {
-//         label l2:
-//         let initial_value = counter.load(SeqCst);
-//         counter.fetch_add(1, SeqCst);
-//         let final_value = counter.load(SeqCst);
-//         assert!(final_value >= initial_value + 1);
-//         i += 1;
-//         *remaining -= 1;
-//     }
-//     assert!(i == 10);
-// }
+// This program shows how to model a program that concurrently increments a counter
+// The encoding used using sequential code and claims.
 
 // A universe of objects playing under LCI rules
 trait Universe {
@@ -31,8 +14,7 @@ trait Universe {
     // We define this to allow a generic object operation (O.join below) to add the object to the universe,
     // without having to check the object invariants.
     predicate globalBaseInv() reads this, content {
-        && (forall o: Object | o in content :: o.universe == this && o as object != this)
-        && (forall o: Object | o in content :: o.triggerAxioms())
+        forall o: Object | o in content :: o.universe == this && o as object != this && o.baseFieldsInv() && o.triggerAxioms()
     }
 
     // Global 1-state invariant: all objects satisfy their individual invariants.
@@ -40,24 +22,25 @@ trait Universe {
         globalBaseInv() && (forall o: Object | o in content :: o.inv())
     }
 
-    // Global 2-state invariant: all old objects satisfy their 2-state invariants and basic properties of legal transitions.
-    twostate predicate globalInv2() reads * {
-        && (forall o: Object | o in old(content) :: o in content && o.inv2())
-        // The following could be `legalTransition`, but it's unnecessarily strong. `baseLegalTransitionsSequence` is enough.
-        //&& baseLegalTransitionsSequence() // NEW
+    // Global transitive 2-state invariant: all old objects satisfy their transitive 2-state invariants.
+    twostate predicate globalSequenceInv2() reads * {
+        && forall o: Object | o in old(content) :: o in content && o.sequenceInv2()
     }
 
-    // This transitive relation describes basic properties of sequences of legal transitions.
-    // This relation does not mention the invariants of the objects. For that, see the `legalTransition` predicate.
+    // Global 2-state invariant: all old objects satisfy their 2-state invariants.
+    twostate predicate globalInv2() reads * {
+        forall o: Object | o in old(content) :: o in content && o.inv2()
+    }
+
     twostate predicate baseLegalTransitionsSequence() reads * {
+        && old(globalBaseInv())
+        && globalBaseInv()
         // The universe only grows
         && old(content) <= content
         // All objects added to the universe weren't allocated in the old state.
         // This allows to satisfy the modifies clause checks on the caller side in a sequence of methods that might
         // modify the universe. For example, the `Havoc` and `Interference` methods.
         && (forall o: Object | o !in old(content) && o in content :: !old(allocated(o)))
-        // Version numbers only increase
-        && (forall o: OwnedObject | o in old(content) :: unchanged(o) || old(o.nonvolatileVersion) <= o.nonvolatileVersion) // Apparently, `unchanged(o) ||` helps Dafny and gives a 2x speedup in some cases.
     }
 
     // This relation describes a sequence of legal transitions, each of which can be performed by a newly created thread
@@ -67,17 +50,15 @@ trait Universe {
     // This definition is needed in the definition of the `Interference` and `Havoc` methods, and in the loop invariants of the `Run` methods.
     twostate predicate legalTransitionsSequence(running: set<Thread>) reads * {
         && baseLegalTransitionsSequence()
-        && old(globalBaseInv())
-        && globalBaseInv()
-        // Old objects must obey their transitive 2-state invariants.
-        // `transitiveInv2` needs to be transitive under the assumption `baseLegalTransitionsSequence`.
-        && (forall o: Object | o in old(content) :: o.transitiveInv2()) // NEW
+        // Version numbers only increase
+        // Updated objects must obey their transitive 2-state invariants.
+        && (forall o: Object | o in old(content) :: unchanged(o) || o.sequenceInv2())
         // Objects cannot change the nonvolatile fields if they are directly owned by threads that cannot run.
         // The 2-state invariant of OwnedObject extends this property to objects that are *transitively* owned by the threads.
         && (forall o: OwnedObject | o in old(content) && old(o.owner) is Thread ::
             // Threads created during a legalTransitionsSequence are allowed to run
             old(o.owner) as Thread !in running && old(allocated(o.owner)) ==> old(o.nonvolatileVersion) == o.nonvolatileVersion
-        ) // NEW
+        )
     }
 
     // A legal transition is one that starts from a good state, preserves the universe invariant, and meets the legality conditions.
@@ -86,15 +67,21 @@ trait Universe {
     twostate predicate legalTransition(running: Thread) reads * {
         && legalTransitionsSequence({running})
         && old(globalInv())
-        && globalBaseInv()
         // The first condition for legality: old objects that change a field must obey their 1- and 2-state invariants.
         && (forall o: Object | o in old(content) :: unchanged(o) || (o.inv() && o.inv2()))
         // The second condition for legality: new objects must satisfy their invariants.
         && (forall o: Object | o in content && o !in old(content) :: o.inv())
     }
 
+    // Transitive LCI soundness: legal transitions are good. This makes use of the admissibility obligations build into Object's.
+    twostate lemma sequenceLci(running: set<Thread>)
+        requires legalTransitionsSequence(running)
+        ensures globalSequenceInv2()
+    {
+        forall o: Object | o in old(content) && o.goodPreAndLegalChangesSequence(running) ensures o.sequenceInv2() { o.sequenceAdmissibility(running); }
+    }
+
     // LCI soundness: legal transitions are good. This makes use of the admissibility obligations build into Object's.
-    // The `ProveTransitiveInv2` lemma is often useful to prove the precondition.
     twostate lemma lci(running: Thread)
         requires legalTransition(running)
         ensures globalInv() && globalInv2()
@@ -117,62 +104,33 @@ trait Universe {
         requires globalInv() && preempting in content
         modifies this, this.content
         ensures globalInv()
-        // Ensuring `globalInv2` would be wrong, because it's not guaranteed to be transitive
-        // Ensure that other threads executed any number of legal transitions
-        ensures legalTransitionsSequence(set t: Thread | t in old(content) && t != preempting)
+        // Ensure that other threads executed any number of legal transitions.
+        // Ensuring `globalInv2` would be wrong, because it's not guaranteed to be transitive.
+        ensures legalTransitionsSequence(set t: Thread | t in old(content) && t != preempting) && globalSequenceInv2()
     {
         // This method could be bodyless. Checking the following implementation is just a consistency check.
         // The verifier will report errors in case `legalTransitionsSequence` is not transitive.
         var steps: int :| 0 <= steps;
-        ProveReflexiveLegalTransitionsSequence(set t: Thread | t in content && t != preempting);
+        sequenceLci({});
         while (steps > 0)
-            invariant globalInv() && legalTransitionsSequence(set t: Thread | t in old(content) && t != preempting)
+            invariant globalInv() && legalTransitionsSequence(set t: Thread | t in old(content) && t != preempting) && globalSequenceInv2()
         {
             // A thread of the environment (if there is any) executes a single legal transition.
             var envThreads: set<Thread> := set t: Thread | t in content && t != preempting;
             if (|envThreads| > 0) {
                 ghost var running: Thread :| running in envThreads;
                 label preTransition:
-                assert forall o: Object | o in old(content) :: o.transitiveInv2(); // (1)
+                assert globalSequenceInv2(); // (1)
                 Havoc();
                 assume legalTransition@preTransition(running);
-                ProveTransitiveInv2@preTransition();
                 lci@preTransition(running);
-                assert forall o: Object | o in old@preTransition(content) :: o.transitiveInv2@preTransition(); // (2)
-                // We cannot call a 3-state lemma to apply the transitivity of `transitiveInv2`, so we have to assume this, checking (1) and (2).
-                assume baseLegalTransitionsSequence() ==> forall o: Object | o in old(content) :: o.transitiveInv2();
+                assert globalSequenceInv2@preTransition(); // (2)
+                // We cannot call a 3-state lemma to apply the transitivity of `forall o: Object ... o.sequenceInv2`, so we have to assume this, checking (1) and (2).
+                assume baseLegalTransitionsSequence() ==> globalSequenceInv2();
             }
             steps := steps - 1;
         }
     }
-
-    // A helper lemma, to be used before the `lci` lemma to prove that a transition only changed nonvolatile fields when allowed by the owner.
-    // TODO: See if this can be merged into `lci` or some 2-state invariant.
-    twostate lemma ProveTransitiveInv2()
-        ensures forall o: Object | o in old(content) ::
-            (o is OwnedObject ==>
-                && unchanged(o)
-                && (forall x: OwnedObject | x in old(o.universe.content) && old(x.owner) == o :: old(x.nonvolatileVersion) == x.nonvolatileVersion && x.owner == o)
-            ) ==> o.transitiveInv2()
-    {
-        forall o: Object | o in old(content) ensures
-            (o is OwnedObject ==>
-                && unchanged(o)
-                && (forall x: OwnedObject | x in old(o.universe.content) && old(x.owner) == o :: old(x.nonvolatileVersion) == x.nonvolatileVersion && x.owner == o)
-            ) ==> o.transitiveInv2()
-        {
-            assert o.triggerAxioms();
-            if (o is OwnedObject) {
-                var ownedObject := o as OwnedObject;
-                if (unchanged(o) && forall x: OwnedObject | x in old(ownedObject.universe.content) && old(x.owner) == ownedObject :: old(x.nonvolatileVersion) == x.nonvolatileVersion && x.owner == ownedObject) {
-                    ownedObject.ProveUnchangedNonvolatileFields();
-                }
-            }
-        }
-    }
-
-    // Consistency check: baseLegalTransitionsSequence should be reflexive.
-    lemma ProveReflexiveBaseLegalTransitionsSequence() ensures baseLegalTransitionsSequence() {}
 
     // Consistency check: baseLegalTransitionsSequence should be transitive.
     method CheckTransitiveBaseLegalTransitionsSequence()
@@ -184,13 +142,6 @@ trait Universe {
         Havoc();
     }
 
-    // Consistency check: assuming globalBaseInv, legalTransitionsSequence should be reflexive.
-    lemma ProveReflexiveLegalTransitionsSequence(running: set<Thread>) ensures globalBaseInv() ==> legalTransitionsSequence(running) {
-        forall o: Object | o in old(content) ensures o.transitiveInv2() {
-            o.ProveReflexiveTransitiveInv2();
-        }
-    }
-
     // Consistency check: legalTransitionsSequence should be transitive.
     method CheckTransitiveLegalTransitionsSequence(running: set<Thread>)
         requires globalInv()
@@ -199,13 +150,15 @@ trait Universe {
     {
         Havoc();
         assume legalTransitionsSequence(running);
-        assert forall o: Object | o in old(content) :: o.transitiveInv2(); // (1)
+        sequenceLci(running);
+        assert globalSequenceInv2(); // (1)
         label mid:
         Havoc();
         assume legalTransitionsSequence@mid(running);
-        assert forall o: Object | o in old@mid(content) :: o.transitiveInv2@mid(); // (2)
-        // We cannot call a 3-state lemma to apply the transitivity of `transitiveInv2`, so we have to assume it, checking (1) and (2).
-        assume baseLegalTransitionsSequence() ==> forall o: Object | o in old(content) :: o.transitiveInv2();
+        sequenceLci@mid(running);
+        assert globalSequenceInv2@mid(); // (2)
+        // We cannot call a 3-state lemma to apply the transitivity of `sequenceInv2`, so we have to assume it, checking (1) and (2).
+        assume baseLegalTransitionsSequence() ==> globalSequenceInv2();
     }
 
     // Consistency check: legalTransitionsSequence should be monotonic w.r.t. adding elements to `running`.
@@ -218,7 +171,7 @@ trait Universe {
     // method SmokeTestHavoc()
     //     requires globalInv()
     //     modifies this, content
-    //     ensures false // TODO: Should fail
+    //     ensures false
     // {
     //     Havoc();
     // }
@@ -226,7 +179,7 @@ trait Universe {
     // method SmokeTestInterference(running: Thread)
     //     requires globalInv() && running in content
     //     modifies this, content
-    //     ensures false // TODO: Should fail
+    //     ensures false
     // {
     //     Interference(running);
     // }
@@ -239,32 +192,14 @@ trait Object {
     // because traits can't have constructors.
     const universe: Universe;
 
-    // Base invariant: we're in the universe, and the universe satisfies its base.
-    predicate baseInv() reads * { this in universe.content && universe.globalBaseInv() }
-
-    // Join the universe
-    method join()
-        requires universe.globalBaseInv() && this as object != universe
-        modifies universe
-        ensures baseInv() && universe.content == old(universe.content) + { this }
-        ensures unchanged(universe.content) // This method doesn't modify fields of objects in the universe
-    {
-        universe.content := universe.content + { this };
-    }
-
-    // Precondition for the admissibility check.
-    // This is broken into a separate predicate because Dafny currently doesn't allow adm.requires() in a 1-state context
-    twostate predicate goodPreAndLegalChanges(running: Thread) reads * {
-        && old(baseInv() && universe.globalInv()) && baseInv() // TODO: this could just be `this in universe.content`. legalTransition implies the rest.
-        && unchanged(this)
-        && universe.legalTransition(running)
-    }
+    // Global base invariant (from o's perspective)
+    predicate objectGlobalBaseInv() reads * { this in universe.content && baseFieldsInv() && universe.globalBaseInv() }
 
     // Global invariant (from o's perspective) - I am in the universe and the universe is good. (This implies I am good also.)
-    predicate objectGlobalInv() reads * { baseInv() && universe.globalInv() }
+    predicate objectGlobalInv() reads * { this in universe.content && universe.globalInv() }
 
     // Global 2-state invariant (from o's perspective).
-    twostate predicate objectGlobalInv2() requires old(objectGlobalInv()) reads *  { baseInv()  && universe.globalInv2() }
+    twostate predicate objectGlobalInv2() requires old(objectGlobalInv()) reads *  { objectGlobalBaseInv()  && universe.globalInv2() }
 
     predicate triggerAxioms() reads this ensures triggerAxioms() {
         assume (this is OwnedObject || this is Thread) && !(this is OwnedObject && this is Thread);
@@ -272,14 +207,43 @@ trait Object {
         && !(this is OwnedObject && this is Thread)
     }
 
+    // Join the universe
+    method join()
+        requires universe.globalBaseInv() && baseFieldsInv() && this as object != universe
+        modifies universe
+        ensures objectGlobalBaseInv() && universe.content == old(universe.content) + { this }
+    {
+        universe.content := universe.content + { this };
+        forall o: Object | o in universe.content ensures o.baseFieldsInv() {
+            o.baseFieldsInvMonotonicity();
+        }
+    }
+
+    // Precondition for the sequence admissibility check.
+    twostate predicate goodPreAndLegalChangesSequence(running: set<Thread>) reads * {
+        && old(this in universe.content)
+        && unchanged(this)
+        && universe.legalTransitionsSequence(running)
+    }
+
+    // Precondition for the admissibility check.
+    // This is broken into a separate predicate because Dafny currently doesn't allow adm.requires() in a 1-state context
+    twostate predicate goodPreAndLegalChanges(running: Thread) reads * {
+        && old(this in universe.content)
+        && unchanged(this)
+        && universe.legalTransition(running)
+    }
+
     // To be implemented: 1-state invariant, 2-state invariant, admissibility proof...
     predicate isOwnedObject() // To prevent a class from extending both OwnedObject and Thread
-    predicate localInv() reads *
+    predicate baseFieldsInv() reads this, universe // All fields of this object are in the universe
+    twostate lemma baseFieldsInvMonotonicity() requires old(baseFieldsInv()) && old(universe.content) <= universe.content && unchanged(this) ensures baseFieldsInv()
+    predicate localInv() reads * ensures localInv() ==> objectGlobalBaseInv()
     twostate predicate localInv2() reads *
     predicate inv() ensures inv() ==> localInv() reads *
-    twostate predicate transitiveInv2() reads * // Assuming universe.baseLegalTransitionsSequence(), this should be transitive. This can be checked with a method. See `CheckTransitiveInv2` below.
-    twostate predicate inv2() ensures inv2() ==> localInv2() && transitiveInv2() reads *
-    lemma ProveReflexiveTransitiveInv2() ensures transitiveInv2()
+    twostate predicate sequenceInv2() reads * // This should be transitive. See `CheckSequenceInv2` below.
+    twostate predicate inv2() ensures inv2() ==> localInv2() && sequenceInv2() reads *
+    twostate lemma sequenceAdmissibility(running: set<Thread>) requires goodPreAndLegalChangesSequence(running) ensures sequenceInv2()
     twostate lemma admissibility(running: Thread) requires goodPreAndLegalChanges(running) ensures inv2() && inv()
 }
 
@@ -287,8 +251,13 @@ class Thread extends Object {
     // To prevent a class from extending both OwnedObject and Thread
     predicate isOwnedObject() { false }
 
+    predicate baseFieldsInv() reads this, universe {
+        true
+    }
+    twostate lemma baseFieldsInvMonotonicity() requires old(baseFieldsInv()) && old(universe.content) <= universe.content && unchanged(this) ensures baseFieldsInv() {}
+
     predicate localInv() reads * {
-        && baseInv()
+        && objectGlobalBaseInv()
     }
     predicate inv() reads * ensures inv() ==> localInv() {
         && localInv()
@@ -297,29 +266,27 @@ class Thread extends Object {
     twostate predicate localInv2() reads * {
         true
     }
-    twostate predicate transitiveInv2() reads * {
+    twostate predicate sequenceInv2() reads * {
         true
     }
-    twostate predicate inv2() reads * ensures inv2() ==> localInv2() && transitiveInv2()  {
-        localInv2() && transitiveInv2()
+    twostate predicate inv2() reads * ensures inv2() ==> localInv2() && sequenceInv2()  {
+        localInv2() && sequenceInv2()
     }
 
-    lemma ProveReflexiveTransitiveInv2() ensures transitiveInv2()
-
+    twostate lemma sequenceAdmissibility(running: set<Thread>) requires goodPreAndLegalChangesSequence(running) ensures sequenceInv2() {}
     twostate lemma admissibility(running: Thread) requires goodPreAndLegalChanges(running) ensures inv2() && inv() {}
 
-    // Check (trivial) transitivity of transitiveInv2()
-    method CheckTransitiveInv2()
+    // Check (trivial) transitivity of sequenceInv2()
+    method CheckSequenceInv2()
         requires objectGlobalInv()
         modifies universe, universe.content
-        ensures transitiveInv2()
+        ensures sequenceInv2()
     {
         universe.Havoc();
-        assume transitiveInv2() && universe.baseLegalTransitionsSequence();
+        assume universe.baseLegalTransitionsSequence() && forall o: Object | o in old(universe.content) :: o.sequenceInv2();
         label mid:
         universe.Havoc();
-        assume transitiveInv2@mid() && universe.baseLegalTransitionsSequence@mid();
-        universe.ProveTransitiveInv2();
+        assume universe.baseLegalTransitionsSequence@mid() && forall o: Object | o in old@mid(universe.content) :: o.sequenceInv2@mid();
     }
 
     // Here we require a thread to create a thread. Programs shold assume that an initial thread exists in the universe.
@@ -331,7 +298,6 @@ class Thread extends Object {
         this.universe := universe;
         new;
         join();
-        universe.ProveTransitiveInv2();
         universe.lci(running);
     }
 }
@@ -347,10 +313,17 @@ trait OwnedObject extends Object {
         old(owner) == owner && unchangedNonvolatileUserFields()
     }
 
-    predicate localInv() reads * {
-        && baseInv()
+    predicate baseFieldsInv() reads this, universe {
         && owner in universe.content
-        && baseUserInv()
+        && baseUserFieldsInv()
+    }
+    twostate lemma baseFieldsInvMonotonicity() requires old(baseFieldsInv()) && old(universe.content) <= universe.content && unchanged(this) ensures baseFieldsInv() {
+        baseUserFieldsInvMonotonicity();
+        assert owner in universe.content;
+    }
+
+    predicate localInv() reads * {
+        && objectGlobalBaseInv()
         && localUserInv()
     }
     predicate inv() reads * ensures inv() ==> localInv() {
@@ -362,15 +335,14 @@ trait OwnedObject extends Object {
         && localUserInv2()
     }
 
-    // Assuming `universe.globalBaseInv2()`, this relation should be transitive.
-    twostate predicate transitiveInv2() reads * {
+    twostate predicate sequenceInv2() reads * {
+        && old(nonvolatileVersion) <= nonvolatileVersion
         && (old(nonvolatileVersion) == nonvolatileVersion ==>
             // Nonvolatile fields are only allowed to change when the nonvolatileVersion changes.
-            // (The ProveTransitiveInv2 lemma should be useful to prove this.)
             // TODO: This could be optimized by making the nonvolatile fields a version of the nonvolatile version number
             && unchangedNonvolatileFields()
             // Transitivity: if a nonvolatileVersion doesn't change, the same should apply to all owned objects
-            && (forall o: OwnedObject | o in old(universe.content) && old(o.owner) == this :: old(o.nonvolatileVersion) == o.nonvolatileVersion && o.owner == this) // FIXME: This might be expensive
+            //&& (forall o: OwnedObject | o in old(universe.content) && old(o.owner) == this :: old(o.nonvolatileVersion) == o.nonvolatileVersion && o.owner == this) // FIXME: This might be expensive
         )
         // The nonvolatileVersion cannot change if the version of the old owner doesn't change.
         && (old(owner) is OwnedObject ==>
@@ -378,16 +350,16 @@ trait OwnedObject extends Object {
             old(oldOwner.nonvolatileVersion) == oldOwner.nonvolatileVersion ==> old(nonvolatileVersion) == nonvolatileVersion
         )
         // The nonvolatileVersion cannot change if the version of the new owner doesn't change.
-        // Note: this seems fine, but unnecessary.
+        // Note: this is inconvenient. Receiving ownership shouldn't require to change the nonvolatile version.
         // && (owner is OwnedObject ==>
         //     var newOwner := owner as OwnedObject;
         //     old(allocated(newOwner)) && old(newOwner.nonvolatileVersion) == newOwner.nonvolatileVersion ==> old(nonvolatileVersion) == nonvolatileVersion
         // )
     }
 
-    twostate predicate inv2() reads * ensures inv2() ==> localInv2() && transitiveInv2() {
+    twostate predicate inv2() reads * ensures inv2() ==> localInv2() && sequenceInv2() {
         && localInv2()
-        && transitiveInv2()
+        && sequenceInv2()
         && userInv2()
         // When the owner changes, the invariant of the old and new owner must hold.
         && (old(owner) != owner ==>
@@ -399,40 +371,31 @@ trait OwnedObject extends Object {
         )
     }
 
-    lemma ProveReflexiveTransitiveInv2() ensures transitiveInv2() {
-        ProveUnchangedNonvolatileFields();
-    }
-
-    // Check transitivity of transitiveInv2()
-    method CheckTransitiveInv2()
+    // Check transitivity of sequenceInv2()
+    method CheckSequenceInv2()
         requires objectGlobalInv()
         modifies universe, universe.content
-        ensures transitiveInv2()
+        ensures sequenceInv2()
     {
         universe.Havoc();
-        assume transitiveInv2() && universe.baseLegalTransitionsSequence();
+        assume universe.baseLegalTransitionsSequence() && forall o: Object | o in old(universe.content) :: o.sequenceInv2();
         var u1 := unchangedNonvolatileFields(); // (1)
         label mid:
         universe.Havoc();
-        assume transitiveInv2@mid() && universe.baseLegalTransitionsSequence@mid();
+        assume universe.baseLegalTransitionsSequence@mid() && forall o: Object | o in old@mid(universe.content) :: o.sequenceInv2@mid();
         var u2 := unchangedNonvolatileFields@mid(); // (2)
         // We cannot call a 3-state lemma to apply the transitivity of `unchangedNonvolatileFields`, so we have to assume it.
         assume u1 && u2 ==> unchangedNonvolatileFields();
-        universe.ProveTransitiveInv2();
-    }
-
-    twostate lemma ProveUnchangedNonvolatileFields() requires unchanged(this) ensures unchangedNonvolatileFields() {
-        ProveUnchangedNonvolatileUserFields();
     }
 
     // To be implemented in the class: 1-state invariant, 2-state invariant, admissibility proof...
+    predicate baseUserFieldsInv() reads this, universe
+    twostate lemma baseUserFieldsInvMonotonicity() requires old(baseUserFieldsInv()) && old(universe.content) <= universe.content && unchanged(this) ensures baseUserFieldsInv()
     twostate predicate unchangedNonvolatileUserFields() reads this // Checking transitivity is up to the classes that implement this trait.
-    predicate baseUserInv() reads *
     predicate localUserInv() reads *
     twostate predicate localUserInv2() reads *
     predicate userInv() reads * ensures userInv() ==> localUserInv()
     twostate predicate userInv2() reads * ensures userInv2() ==> localUserInv2()
-    twostate lemma ProveUnchangedNonvolatileUserFields() requires unchanged(this) ensures unchangedNonvolatileUserFields()
 
     // Every class should check the transitivity of unchangedNonvolatileFields():
     // method CheckTransitiveUnchangedNonvolatileFields()
@@ -449,55 +412,14 @@ trait OwnedObject extends Object {
 
 method BumpVersion(ghost last: int) returns (res: int) ensures res > last
 
-// An example of type without fields
-class EmptyType extends OwnedObject {
-    twostate predicate unchangedNonvolatileUserFields() reads this { true }
-    twostate lemma ProveUnchangedNonvolatileUserFields() requires unchanged(this) ensures unchangedNonvolatileUserFields() {}
-
-    predicate baseUserInv() reads * { true }
-
-    predicate localUserInv() reads * { true }
-    predicate userInv() reads * ensures userInv() ==> localUserInv() { localUserInv() }
-    twostate predicate localUserInv2() reads * { true }
-    twostate predicate userInv2() reads * ensures userInv2() ==> localUserInv2() { localUserInv2() }
-
-    twostate lemma admissibility(running: Thread) requires goodPreAndLegalChanges(running) ensures inv2() && inv() {}
-
-    // method SmokeTestTransitiveInv2()
-    //     requires objectGlobalInv()
-    //     modifies universe, universe.content
-    //     ensures false // TODO: Should fail
-    // {
-    //     universe.Havoc();
-    //     assume transitiveInv2() && universe.baseLegalTransitionsSequence();
-    // }
-
-    constructor(universe: Universe, ghost running: Thread)
-        requires universe.globalInv() && running in universe.content
-        modifies universe
-        ensures objectGlobalInv() && universe.globalInv2()
-        ensures this.universe == universe && this.owner == running
-        ensures universe.content == old(universe.content)  + { this }
-    {
-        this.universe := universe;
-        this.owner := running;
-        new;
-        join();
-        universe.ProveTransitiveInv2();
-        universe.lci(running);
-    }
-}
-
 // A strictly increasing counter
 class IncreasingCounter extends OwnedObject {
     var value: int; // volatile
 
-    twostate predicate unchangedNonvolatileUserFields() reads this { true }
-    twostate lemma ProveUnchangedNonvolatileUserFields() requires unchanged(this) ensures unchangedNonvolatileUserFields() {}
+    predicate baseUserFieldsInv() reads this, universe { true }
+    twostate lemma baseUserFieldsInvMonotonicity() requires old(baseUserFieldsInv()) && old(universe.content) <= universe.content && unchanged(this) ensures baseUserFieldsInv() {}
 
-    predicate baseUserInv() reads * {
-        && true
-    }
+    twostate predicate unchangedNonvolatileUserFields() reads this { true }
 
     predicate localUserInv() reads * {
         && true
@@ -513,12 +435,14 @@ class IncreasingCounter extends OwnedObject {
         && localUserInv2()
     }
 
+    twostate lemma sequenceAdmissibility(running: set<Thread>) requires goodPreAndLegalChangesSequence(running) ensures sequenceInv2() {}
     twostate lemma admissibility(running: Thread) requires goodPreAndLegalChanges(running) ensures inv2() && inv() {}
 
     constructor(universe: Universe, ghost running: Thread, value: int)
         requires universe.globalInv() && running in universe.content
         modifies universe
         ensures objectGlobalInv() && universe.globalInv2()
+        // The following might not always be needed
         ensures this.universe == universe && this.owner == running && this.value == value
         ensures universe.content == old(universe.content)  + { this }
     {
@@ -527,7 +451,6 @@ class IncreasingCounter extends OwnedObject {
         this.owner := running;
         new;
         join();
-        universe.ProveTransitiveInv2();
         universe.lci(running);
     }
 }
@@ -535,13 +458,11 @@ class IncreasingCounter extends OwnedObject {
 class Integer extends OwnedObject {
     var value: int; // nonvolatile
 
+    predicate baseUserFieldsInv() reads this, universe { true }
+    twostate lemma baseUserFieldsInvMonotonicity() requires old(baseUserFieldsInv()) && old(universe.content) <= universe.content && unchanged(this) ensures baseUserFieldsInv() {}
+
     twostate predicate unchangedNonvolatileUserFields() reads this {
         old(value) == value
-    }
-    twostate lemma ProveUnchangedNonvolatileUserFields() requires unchanged(this) ensures unchangedNonvolatileUserFields() {}
-
-    predicate baseUserInv() reads * {
-        && true
     }
 
     predicate localUserInv() reads * {
@@ -558,12 +479,14 @@ class Integer extends OwnedObject {
         && localUserInv2()
     }
 
+    twostate lemma sequenceAdmissibility(running: set<Thread>) requires goodPreAndLegalChangesSequence(running) ensures sequenceInv2() {}
     twostate lemma admissibility(running: Thread) requires goodPreAndLegalChanges(running) ensures inv2() && inv() {}
 
     constructor(universe: Universe, ghost running: Thread, value: int)
         requires universe.globalInv() && running in universe.content
         modifies universe
         ensures objectGlobalInv() && universe.globalInv2()
+        // The following might not always be needed
         ensures this.universe == universe && this.owner == running && this.value == value
         ensures universe.content == old(universe.content) + { this }
     {
@@ -572,7 +495,6 @@ class Integer extends OwnedObject {
         this.owner := running;
         new;
         join();
-        universe.ProveTransitiveInv2();
         universe.lci(running);
     }
 }
@@ -580,13 +502,11 @@ class Integer extends OwnedObject {
 class ConstantInteger extends OwnedObject {
     var value: int; // nonvolatile
 
+    predicate baseUserFieldsInv() reads this, universe { true }
+    twostate lemma baseUserFieldsInvMonotonicity() requires old(baseUserFieldsInv()) && old(universe.content) <= universe.content && unchanged(this) ensures baseUserFieldsInv() {}
+
     twostate predicate unchangedNonvolatileUserFields() reads this {
         old(value) == value
-    }
-    twostate lemma ProveUnchangedNonvolatileUserFields() requires unchanged(this) ensures unchangedNonvolatileUserFields() {}
-
-    predicate baseUserInv() reads * {
-        && true
     }
 
     predicate localUserInv() reads * {
@@ -603,6 +523,7 @@ class ConstantInteger extends OwnedObject {
         && localUserInv2()
     }
 
+    twostate lemma sequenceAdmissibility(running: set<Thread>) requires goodPreAndLegalChangesSequence(running) ensures sequenceInv2() {}
     twostate lemma admissibility(running: Thread) requires goodPreAndLegalChanges(running) ensures inv2() && inv() {}
 
     constructor(universe: Universe, ghost running: Thread, value: int)
@@ -618,7 +539,6 @@ class ConstantInteger extends OwnedObject {
         this.owner := running;
         new;
         join();
-        universe.ProveTransitiveInv2();
         universe.lci(running);
     }
 }
@@ -627,14 +547,14 @@ class ClaimIncreasingCounterGreaterThanConstant extends OwnedObject {
     var counter: IncreasingCounter; // nonvolatile
     var constant: ConstantInteger; // nonvolatile
 
-    twostate predicate unchangedNonvolatileUserFields() reads this {
-        old(counter) == counter && old(constant) == constant
-    }
-    twostate lemma ProveUnchangedNonvolatileUserFields() requires unchanged(this) ensures unchangedNonvolatileUserFields() {}
-
-    predicate baseUserInv() reads * {
+    predicate baseUserFieldsInv() reads this, universe {
         && counter in universe.content
         && constant in universe.content
+    }
+    twostate lemma baseUserFieldsInvMonotonicity() requires old(baseUserFieldsInv()) && old(universe.content) <= universe.content && unchanged(this) ensures baseUserFieldsInv() {}
+
+    twostate predicate unchangedNonvolatileUserFields() reads this {
+        old(counter) == counter && old(constant) == constant
     }
 
     predicate localUserInv() reads * {
@@ -652,6 +572,7 @@ class ClaimIncreasingCounterGreaterThanConstant extends OwnedObject {
         && localUserInv2()
     }
 
+    twostate lemma sequenceAdmissibility(running: set<Thread>) requires goodPreAndLegalChangesSequence(running) ensures sequenceInv2() {}
     twostate lemma admissibility(running: Thread) requires goodPreAndLegalChanges(running) ensures inv2() && inv() {}
 
     constructor(universe: Universe, ghost running: Thread, counter: IncreasingCounter, constant: ConstantInteger)
@@ -659,6 +580,7 @@ class ClaimIncreasingCounterGreaterThanConstant extends OwnedObject {
         requires counter.value >= constant.value
         modifies universe
         ensures objectGlobalInv() && universe.globalInv2()
+        // The following might not always be needed
         ensures this.universe == universe && this.owner == running && this.counter == counter && this.constant == constant
         ensures universe.content == old(universe.content) + { this }
     {
@@ -668,17 +590,19 @@ class ClaimIncreasingCounterGreaterThanConstant extends OwnedObject {
         this.constant := constant;
         new;
         join();
-        universe.ProveTransitiveInv2();
         universe.lci(running);
     }
 }
 
+// Note: the translation from Rust types to Dafny is done manually, in this file. For example, all Rust primitive types
+// should have been translated to a Dafny class in order to allow specifying an owner.
+//
 // fn incrementer(counter: Arc<AtomicIsize>, remaining: &mut isize)
 //   requires *remaining == 10
 //   ensures *remaining == 0
 // {
 //     let mut i = 0;
-//     while i < 10 {
+//     while {:... } i < 10 {
 //         label l2:
 //         let initial_value = counter.load(SeqCst);
 //         counter.fetch_add(1, SeqCst);
@@ -701,7 +625,6 @@ method Incrementer(universe: Universe, running: Thread, counter: IncreasingCount
 
     label l0:
     var i := 0;
-    universe.ProveTransitiveInv2@l0();
     universe.lci@l0(running);
 
         universe.Interference(running);
@@ -717,21 +640,18 @@ method Incrementer(universe: Universe, running: Thread, counter: IncreasingCount
         label l2:
         var initial_value := new ConstantInteger(universe, running, counter.value);
         var claim1 := new ClaimIncreasingCounterGreaterThanConstant(universe, running, counter, initial_value);
-        universe.ProveTransitiveInv2@l2();
         universe.lci@l2(running);
 
             universe.Interference(running);
 
         label l3:
         counter.value := counter.value + 1;
-        universe.ProveTransitiveInv2@l3();
         universe.lci@l3(running);
         
             // No interference!
 
         label l3p1:
         var initial_value_plus_one := new ConstantInteger(universe, running, initial_value.value + 1);
-        universe.ProveTransitiveInv2@l3p1();
         universe.lci@l3p1(running);
         
             // No interference!
@@ -740,7 +660,6 @@ method Incrementer(universe: Universe, running: Thread, counter: IncreasingCount
         // assert claim1.inv(); // Help Dafny (1)
         // assert {:split_here} claim1.counter == counter && claim1.constant == initial_value; // Help Dafny (1)
         var claim2 := new ClaimIncreasingCounterGreaterThanConstant(universe, running, counter, initial_value_plus_one);
-        universe.ProveTransitiveInv2@l3p2();
         universe.lci@l3p2(running);
 
             universe.Interference(running);
@@ -749,7 +668,6 @@ method Incrementer(universe: Universe, running: Thread, counter: IncreasingCount
         // assert claim2.inv(); // Help Dafny (1)
         // assert {:split_here} claim2.counter == counter && claim2.constant == initial_value_plus_one; // Help Dafny (1)
         var final_value := new ConstantInteger(universe, running, counter.value);
-        universe.ProveTransitiveInv2@l4();
         universe.lci@l4(running);
 
             universe.Interference(running);
@@ -760,16 +678,14 @@ method Incrementer(universe: Universe, running: Thread, counter: IncreasingCount
         // assert claim1.counter == counter && claim1.constant == initial_value; // Help Dafny (1)
         // assert claim2.counter == counter && claim2.constant == initial_value_plus_one; // Help Dafny (1)
         // assert initial_value_plus_one.value == initial_value.value + 1; // Help Dafny (1)
-        assert final_value.value >= initial_value.value + 1;
+        // assert final_value.value >= initial_value.value + 1; // Help Dafny (1)
         assert {:split_here} true;
-        universe.ProveTransitiveInv2@l5();
         universe.lci@l5(running);
 
             universe.Interference(running);
 
         label l6:
         i := i + 1;
-        universe.ProveTransitiveInv2@l6();
         universe.lci@l6(running);
 
             universe.Interference(running);
@@ -783,24 +699,18 @@ method Incrementer(universe: Universe, running: Thread, counter: IncreasingCount
         remaining.nonvolatileVersion := BumpVersion(remaining.nonvolatileVersion);
         assert {:split_here} remaining.inv2@l7(); // Help Dafny?
         assert {:split_here} universe.baseLegalTransitionsSequence@l7(); // Help Dafny?
-        universe.ProveTransitiveInv2@l7();
         assert {:split_here} universe.legalTransitionsSequence@l7({running}); // Help Dafny?
         assert {:split_here} universe.legalTransition@l7(running); // Help Dafny?
         universe.lci@l7(running);
 
             universe.Interference(running);
-
-        // assert false; // Smoke test
     }
 
         universe.Interference(running);
 
     label l8:
     assert i == 10;
-    universe.ProveTransitiveInv2@l8();
     universe.lci@l8(running);
 
         universe.Interference(running);
-
-    // assert false; // Smoke test
 }
